Start rewrite of stack machine types

sml.v
@@ -9,191 +9,238 @@ Load lambda.
 
 Module SML.
 
-  Inductive Item : Set :=
-  | item_nat : nat -> Item
-  | item_tuple : list Item -> Item.
+  (* TODO: stack_equiv showing empty and singleton tuples can be reduced *)
+  Inductive Stack: Set :=
+  | snil
+  | snat (n: nat) (s: Stack)
+  | stuple (t: Stack) (s: Stack).
 
-  Inductive SMProgram : Set :=
-  | sm_end : SMProgram
-  | push : nat -> SMProgram -> SMProgram
-  | pop : SMProgram -> SMProgram
-  | get : nat -> SMProgram -> SMProgram
-  (*| rotate : nat -> SMProgram -> SMProgram *)
-  | pack : nat -> SMProgram -> SMProgram
-  | unpack : SMProgram -> SMProgram
-  | call : SMProgram -> SMProgram
-  | out : SMProgram -> SMProgram.
+  Inductive SMCommand : Set :=
+  | push (n: nat)
+  | del (n: nat)
+  | get (n: nat)
+  | pack (n: nat)
+  | unpack
+  | call
+  | out.
 
-
-  Definition Stack := list Item.
+  Definition SMProgram := list SMCommand.
 
   Inductive SMState :=
-    | running (ast: SMProgram)
-          (to_return: list SMProgram)
+    | running (smp: SMProgram)
+          (returns: list SMProgram)
           (fn_table: list SMProgram)
           (stack: Stack)
           (output: list nat)
+    | halted (output: list nat)
+    | error.
 
-    | error (output: list nat)
-    | halted (output: list nat).
-
-  Definition failsafe_tl {A: Type} (l: list A) :=
-    match l with
-    | [] => []
-    | _ :: tl => tl
-    end.
-
-  Definition tl_error {A} (l : list A) : option (list A) :=
-    match l with
-    | [] => None
-    | _ :: tl => Some tl
-    end.
-
-  Definition hd_error {A} (l : list A) : option A :=
-    match l with
-    | [] => None
-    | hd :: _ => Some hd
-    end.
-
-  Fixpoint stack_pack (n : nat) (s: Stack) :=
-  match n with
-  | 0 | S 0=> Some s
-  | S (S 0) => match s with
-    | l :: k :: tl => Some ((item_tuple (l :: [k])) :: tl)
-    | _ => None
-    end
-  | S n => (stack_pack n s) >>= (fun s =>
-    match s with
-    | item_tuple l :: k :: tl => Some ((item_tuple (l ++ [k])) :: tl)
-    | _ => None
-    end)
-  end.
-
-  Example stack_pack_simple:
-    stack_pack 2 [item_nat 0; item_nat 1] = Some [item_tuple [item_nat 0; item_nat 1]].
-  Proof. simpl. auto. Qed.
-  
-  Eval compute in stack_pack 2 ([item_tuple [item_nat 0; item_nat 1]; item_nat 2; item_nat 3;
-         item_nat 4]).
-  
-  Fixpoint stack_unpack (s: Stack) :=
-    match s with
-    | [] => None
-    | hd :: tl => match hd with
-      | item_nat _ => None
-      | item_tuple lst => Some (lst ++ tl)
+  Function stack_del (n: nat) (s: Stack): option Stack :=
+    match (s, n) with
+    | (snil, _) => None
+    | (snat _ s, 0)
+    | (stuple _ s, 0) => Some s
+    | (snat m s, S n) =>
+      match stack_del n s with
+      | None => None
+      | Some s' => Some (snat m s')
+      end
+    | (stuple t s, S n) =>
+      match stack_del n s with
+      | None => None
+      | Some s' => Some (stuple t s')
       end
     end.
 
-  (*Lemma stack_pack_unpack (s s': Stack) (n: nat):
-    n > 0 ->
-    (stack_pack n s) = Some s' ->
-    (stack_pack n s) >>= stack_unpack = Some s.
-  Proof.
-  Admitted.*)
-
-  Definition sm_bind {A : Type} (a: option A) (f : A -> SMState) (output: list nat) :=
-    match a with
-    | None => error output
-    | Some a => f a
+  Function stack_postfix (n: nat) (s: Stack): option Stack :=
+    match n with
+    | 0 => Some s
+    | S n' =>
+      match s with
+      | snil => None
+      | snat _ s'
+      | stuple _ s' => stack_postfix n' s'
+      end
     end.
+
+  Function stack_get (n: nat) (s: Stack): option Stack :=
+    match stack_postfix n s with
+    | None | Some snil => None
+    | Some (snat m _) => Some (snat m s)
+    | Some (stuple t _) => Some (stuple t s)
+    end.
+
+  Function stack_prefix (n: nat) (s: Stack): option Stack :=
+    match n with
+    | 0 => Some snil
+    | S n' =>
+      match s with
+      | snil => None
+      | snat m s =>
+        match stack_prefix n' s with
+        | None => None
+        | Some s' => Some (snat m s')
+        end
+      | stuple t s =>
+        match stack_prefix n' s with
+        | None => None
+        | Some s' => Some (stuple t s')
+        end
+      end
+    end.
+
+  Example stack_prefix_ex:
+    forall s, stack_prefix 1 (snat 3 s) = Some (snat 3 snil).
+  Proof. intros; auto. Qed.
+
+  Function stack_pack (n: nat) (s: Stack): option Stack :=
+    match n with
+    | 0 | 1 => Some s
+    | _ =>
+      match (stack_prefix n s, stack_postfix n s) with
+      | (Some t, Some s') => Some (stuple t s')
+      | _ => None
+      end
+    end.
+
+  Example stack_pack_simple:
+    stack_pack 2 (snat 0 (snat 1 snil)) =
+    Some (stuple (snat 0 (snat 1 snil)) snil).
+  Proof. auto. Qed.
+
+  Example stack_pack_nested:
+    forall tl,
+      stack_pack 3 (snat 1
+                         (stuple (snat 2 (snat 3 snil))
+                                 (snat 4 tl))) =
+      Some (stuple (snat 1
+                         (stuple (snat 2 (snat 3 snil))
+                                 (snat 4 snil)))
+                   tl).
+  Proof. intros; auto. Qed.
+
+  (* TODO: implement stack_unpack *)
+  Function stack_unpack (s: Stack): option Stack :=
+    None.
+
+  Function stack_weight (s: Stack): nat :=
+    match s with
+    | snil => 0
+    | snat _ s' => S (stack_weight s')
+    | stuple t s' => S (stack_weight t + stack_weight s')
+    end.
+
+  Function stack_call (s: Stack) (fn_table: list SMProgram)
+           {measure stack_weight s}: (option Stack) * SMProgram :=
+    match stack_unpack s with
+    | None => (None, [])
+    | Some stack =>
+      match stack with
+      | snil => (None, [])
+      | stuple t s' => stack_call stack fn_table
+      | snat fid s' =>
+        match nth_error fn_table fid with
+        | None => (None, [])
+        | Some fn => (Some s', fn)
+        end
+      end
+    end.
+  Proof.
+    intros; inversion teq.
+  Defined.
+
+  (* TODO: implement stack_out *)
+  Function stack_out (s: Stack): (option Stack) * nat :=
+    (None, 0).
 
   Definition sm_step (s: SMState): SMState :=
     match s with
-    | halted _ => s
-    | error _ => s
-    | running smp ret_list fn_table stack output =>
-      let state_from_stack (smp': SMProgram) (stack : Stack) :=
-        running smp' ret_list fn_table stack output
-      in match smp with
-      | sm_end => match ret_list with
-        | [] => halted output
-        | smp' :: tl => running smp' tl fn_table stack output
+    | halted _ | error => s
+    | running smp rets fn_table stack output =>
+      match smp with
+      | [] =>
+        match rets with
+        | smp' :: rets' => running smp' rets' fn_table stack output
+        | _ => halted output
         end
-      | push n smp' => state_from_stack smp' ((item_nat n) :: stack)
-      | pop smp'=> sm_bind (tl_error stack) (state_from_stack smp') output
-      | get n smp' =>
-        let new_stack := (nth_error stack n) >>= (fun a => Some (a :: stack))
-        in sm_bind new_stack (state_from_stack smp') output
-      | pack n smp' => sm_bind (stack_pack n stack) (state_from_stack smp') output
-      | unpack smp' => sm_bind (stack_unpack stack) (state_from_stack smp') output
-      | call smp' => match stack with
-        | (item_nat id) :: tl => sm_bind (nth_error fn_table id) 
-            (fun smp => running smp (smp' :: ret_list) fn_table tl output) output
-        | _ => error output
+      | push n :: smp' =>
+        running smp' rets fn_table (snat n stack) output
+      | del n :: smp' =>
+        match stack_del n stack with
+        | Some stack' => running smp' rets fn_table stack' output
+        | None => error
         end
-      | out smp' => let out_char := 
-        match stack with
-        | (item_nat o) :: _ => Some o
-        | _ => None
-        end in 
-        sm_bind out_char (fun o => running smp' ret_list fn_table stack (o :: output)) output
+      | get n :: smp' =>
+        match stack_get n stack with
+        | Some stack' => running smp' rets fn_table stack' output
+        | None => error
+        end
+      | pack n :: smp' =>
+        match stack_pack n stack with
+        | Some stack' => running smp' rets fn_table stack' output
+        | None => error
+        end
+      | unpack :: smp' =>
+        match stack_unpack stack with
+        | Some stack' => running smp' rets fn_table stack' output
+        | None => error
+        end
+      | call :: smp' =>
+        match stack_call stack fn_table with
+        | (Some stack', smf) =>
+          running smf (smp' :: rets) fn_table stack' output
+        | (None, _) => error
+        end
+      | out :: smp' =>
+        match stack_out stack with
+        | (Some stack', a) => running smp' rets fn_table stack' (output ++ [a])
+        | (None, _) => error
+        end
       end
     end.
 
-  (* TODO: Abstract the functions below along with the stuff in bftape.v *)
-  Definition exec_output (state: SMState): list nat :=
-    match state with 
-    | running _ _ _ _ output => output 
-    | halted output => output
-    | error output => output
+  Definition exec_init (main: SMProgram) (fn_table: list SMProgram) : SMState :=
+    running main [] fn_table snil [].
+
+  Definition interpret (main: SMProgram) (fn_table: list SMProgram) (fuel: nat):
+    option (list nat) :=
+    match Utils.run sm_step (exec_init main fn_table) fuel with
+    | halted output => Some output
+    | _ => None
     end.
 
-  Definition exec_init (fn_table: list SMProgram) : SMState :=
-    match fn_table with
-    | smp :: _ => running smp [] fn_table [] []
-    | [] => error []
-    end.
+  (* Example push_simple: *)
+  (*   interpret [push 3; out] [] 20 = Some [3]. *)
+  (* Proof. auto. Qed. *)
 
-  Definition interpret (fn_table: list SMProgram) (fuel: nat): list nat :=
-    exec_output (Utils.run sm_step (exec_init fn_table) fuel). 
+  (* Example call_simple: *)
+  (*   interpret [push 0; out; call; push 2; out] [push 3; out;] 20 = [0; 3; 2]. *)
+  (* Proof. auto. Qed. *)
 
-  Example push_simple:
-    interpret [push 3 (out sm_end)] 20 = [3].
-  Proof. auto. Qed.
+  (* Definition stack_diff (smp: SMProgram) : nat := *)
+  (*   0. *)
 
-  Example jump_simple:
-    interpret [push 1 (out (call (push 2 (out sm_end)))); push 3 (out sm_end)] 20 = [2; 3; 1].
-  Proof. auto. Qed.
+  (* Function lambda_to_sml (l: Lambda.Lambda) (fn_table: list SMProgram) *)
+  (*          (depth: nat) : SMProgram * list SMProgram := *)
+  (*   match l with *)
+  (*   | Lambda.var n => let known_stack_size := 3 in *)
+  (*     ((get (known_stack_size - n) sm_end), fn_table) *)
+  (*   | Lambda.lam e => let (body, c1) := lambda_to_sml e fn_table (depth + 1) in *)
+  (*     let diff := (stack_diff body) + depth in *)
+  (*     let fn := body ++ (pack diff sm_end) in *)
+  (*     (push (List.length c1) sm_end, c1 ++ [fn]) *)
+  (*   | Lambda.app e1 e2 => *)
+  (*     let (f, c1) := lambda_to_sml e1 fn_table depth in *)
+  (*     let (v, c2) := lambda_to_sml e2 c1 depth in *)
+  (*     ((v ++ f) ++ (unpack (call sm_end)), c2) *)
+  (*   | Lambda.out e => let (body, c) := lambda_to_sml e fn_table depth in *)
+  (*     (body ++ (out sm_end), c) *)
+  (*   end. *)
 
-
-  Fixpoint append (sm1 sm2: SMProgram) : SMProgram :=
-    match sm1 with
-    | sm_end => sm2
-    | push n smp' => push n (append smp' sm2) 
-    | pop smp' => pop (append smp' sm2)
-    | get n smp' => get n (append smp' sm2)
-    | pack n smp' => pack n (append smp' sm2)
-    | unpack smp' => unpack (append smp' sm2)
-    | call smp' => call (append smp' sm2)
-    | out smp' => out (append smp' sm2)
-    end.
-
-  Definition stack_diff (smp: SMProgram) : nat :=
-    0.
-
-Notation "s1 +++ s2" := (append s1 s2) (at level 50, left associativity).
-
- Fixpoint lambda_to_sml (l : Lambda.Lambda) (fn_table: list SMProgram) (depth: nat) : SMProgram * list SMProgram :=
-    match l with
-    | Lambda.var n => let known_stack_size := 3 in
-      ((get (known_stack_size - n) sm_end), fn_table)
-    | Lambda.lam e => let (body, c1) := lambda_to_sml e fn_table (depth + 1) in
-      let diff := (stack_diff body) + depth in
-      let fn := body +++ (pack diff sm_end) in
-      (push (List.length c1) sm_end, c1 ++ [fn])
-    | Lambda.app e1 e2 => 
-      let (f, c1) := lambda_to_sml e1 fn_table depth in
-      let (v, c2) := lambda_to_sml e2 c1 depth in
-      ((v +++ f) +++ (unpack (call sm_end)), c2)
-    | Lambda.out e => let (body, c) := lambda_to_sml e fn_table depth in
-      (body +++ (out sm_end), c)
-    end.
-
-  Eval compute in (Lambda.parse_lambda "(\y.\x.x)(\x.x)").
-  Eval compute in (match (Lambda.parse_lambda "(\y. \x.x) (\x. x)") with
-      | Some x => lambda_to_sml x [] 0
-      | None => (sm_end, [])
-      end).
+  (* Eval compute in (Lambda.parse_lambda "(\y.\x.x)(\x.x)"). *)
+  (* Eval compute in (match (Lambda.parse_lambda "(\y. \x.x) (\x. x)") with *)
+  (*     | Some x => lambda_to_sml x [] 0 *)
+  (*     | None => (sm_end, []) *)
+  (*     end). *)
 
 End SML.
