utils.v
@@ -13,7 +13,7 @@ Module Utils.
     | S f => run step (step state) f
     end.
 
-   (* Monads ftw! *)
+  (* Monads ftw! *)
   Definition bind {A B : Type} (a: option A) (f : A -> option B) :=
     match a with
     | None => None
